Automation of simple local regexes without variables.

compiler/regex/ReflexEcho.v
@@ -1,11 +1,14 @@
 Require Import String.
 
 Require Import Reflex.
+Require Import ReflexFin.
 Require Import ReflexBase.
 Require Import ReflexDenoted.
 Require Import ReflexVec.
 Require Import Regex.
 Require Import Ynot.
+Require Import List.
+Require Import Eqdep.
 
 Definition NB_MSG : nat := 1.
 
@@ -29,17 +32,131 @@ Definition HANDLERS : @handler NB_MSG PDV :=
   )
 .
 
-Definition send_star NB_MSG PDV :=
-  RE_Star (RE_Alt (RE_Atom (@KOSend NB_MSG PDV None None))
-                  (RE_Atom (@KOExec NB_MSG PDV None None None))).
+Definition send_star :=
+  RE_Star (RE_Alt (RE_Atom (@KOSelect NB_MSG PDV None None))
+                  (RE_Alt (RE_Atom (@KORecv NB_MSG PDV None None))
+                          (RE_Alt (RE_Atom (@KOSend NB_MSG PDV None None))
+                                  (RE_Alt (RE_Atom
+                                             (@KOExec NB_MSG PDV None None None))
+                                          (RE_Atom
+                                             (@KOBogus NB_MSG PDV None None)))))).
+
+Definition echo_re :=
+  RE_Star
+    (RE_Alt
+       (RE_NAtom (@KOSend NB_MSG PDV None
+                          (Some (@Build_opt_msg NB_MSG PDV
+                                                None (None, tt)))))
+       (RE_Concat
+          (RE_Atom (@KOSend NB_MSG PDV None
+                            (Some (@Build_opt_msg NB_MSG PDV
+                                                  None (None, tt)))))
+          (RE_Atom (@KORecv NB_MSG PDV None
+                            (Some (@Build_opt_msg NB_MSG PDV
+                                                  None (None, tt))))))).
 
 Ltac unpack :=
   match goal with
+  | [ s : kstate, H : ?s = _ |- _ ]
+      (*This is problematic because it destroys information about s*)
+      => apply f_equal with (f:=ktr) in H; rewrite H in *;
+         simpl in *; unpack
   | [ H: [_]%inhabited = [_]%inhabited |- _ ] =>
     apply pack_injective in H;
     rewrite -> H in * || rewrite <- H in *
   end.
 
+Ltac computeMsgMatch NUM_MSG :=
+  match goal with
+  | [ |- context[msgMatch _ _] ]
+    => unfold msgMatch; unfold msgMatch';
+       simpl; computeMsgMatch NUM_MSG
+  | [ |- context[match fin_eq_dec ?fin1 ?fin2 with
+                 | left _ => _ | right _ => _ end] ]
+    => destruct (@fin_eq_dec NUM_MSG fin1 fin2) as [ ?Heq | ?Hneq ];
+       [ assert (Heq = eq_refl fin1) as ?F by apply UIP_refl;
+         rewrite F; compute; intuition
+       | intuition ]
+  end.
+
+Ltac printCtxt :=
+  repeat (match goal with [ H: _ |- _ ] => revert H end);
+  match goal with |- ?G => idtac G end.
+
+Ltac matchAtom NUM_MSG :=
+  match goal with
+  | [ |- RMatch (RE_Atom _) (_::nil) ]
+      => apply RM_Atom; constructor; auto; matchAtom NUM_MSG
+  | [ |- RMatch (RE_NAtom _) (_::nil) ]
+      => apply RM_NAtom; unfold not; inversion 1; matchAtom NUM_MSG
+  | [ |- context G[msgMatch _ _ ] ]
+      => computeMsgMatch NUM_MSG
+  | [ H : msgMatch _ _ |- _ ]
+      => revert H; computeMsgMatch NUM_MSG
+  end.
+
+Ltac matchRE NUM_MSG :=
+  match goal with
+  | [ |- RMatch (RE_Atom _) (_::nil) ]
+      => solve [ matchAtom NUM_MSG ]
+  | [ |- RMatch (RE_NAtom _) (_::nil) ]
+      => solve [ matchAtom NUM_MSG ]
+  | [ |- RMatch (RE_Alt _ _) _ ]
+      => constructor; (left; matchRE NUM_MSG) || (right; matchRE NUM_MSG)
+  | [ |- RMatch (RE_Concat _ _) (_ ++ _) ]
+      => constructor; matchRE NUM_MSG
+  | [ |- RMatch (RE_Star _) (_ ++ _) ]
+      => constructor; matchRE NUM_MSG
+  | [ |- RMatch (RE_Star _) nil ]
+      => solve [constructor]
+
+  (*If there are no matches, we may need to get the trace
+    into the right form by breaking it into two lists.*)
+  | [ |- RMatch _ (?tr1 ++ ?act1::?tr2) ]
+      => replace (tr1 ++ act1::tr2) with
+         ((tr1 ++ (act1::nil)) ++ tr2) by reflexivity;
+         simpl (tr1 ++ (act1::nil)); matchRE NUM_MSG
+  | [ |- RMatch _ (?act::?tl) ]
+      => replace (act::tl) with
+         ((act::nil) ++ tl) by reflexivity; matchRE NUM_MSG
+
+  (*If all else fails, hopefully the goal follows easily from
+    the context.*)
+  | [ |- RMatch _ _ ]
+      => solve [auto]
+  end.
+
+Ltac destruct_msg :=
+  match goal with
+  (*Tag is Some False*)
+  | [ f : False |- _ ]
+      => destruct f
+  | [ pay : s[[lkup_tag _]] |- _ ]
+      => destruct pay; simpl in *
+  | [ tag : fin _ |- _ ]
+      => destruct tag; destruct_msg
+  | [ m : msg |- _ ]
+      => destruct m; destruct_msg
+  end.
+
 Theorem always_send : forall st tr,
   Reach HANDLERS st -> inhabits tr = ktr st ->
-  RMatch (send_star NB_MSG PDV) tr.
+  RMatch send_star tr.
+Proof.
+  intros.
+  unfold send_star.
+  generalize dependent tr.
+  induction H; intros; simpl in *;
+  try destruct_msg; unpack; matchRE NB_MSG.
+Qed.
+
+Theorem echo : forall st tr,
+  Reach HANDLERS st -> inhabits tr = ktr st ->
+  RMatch echo_re tr.
+Proof.
+  intros.
+  unfold echo_re.
+  generalize dependent tr.
+  induction H; intros; simpl in *;
+  try destruct_msg; unpack; matchRE NB_MSG.
+Qed.
